theories/compiler/linearize.v
@@ -1,0 +1,356 @@
+Require Export iris.algebra.lib.gmap_view.
+Require Export refframe.module.
+Require Import refframe.trefines.
+Require Import refframe.filter.
+Require Import refframe.product.
+Require Import refframe.seq_product.
+Require Import refframe.link.
+Require Import stdpp.pretty.
+Require Import refframe.prepost.
+Require Import refframe.proof_techniques.
+Require Import refframe.imp.
+Require Export refframe.compiler.monad.
+Require Export refframe.compiler.linear_imp.
+
+Local Open Scope Z_scope.
+Set Default Proof Using "Type".
+
+Definition tmp_var (n : N) : string :=
+  "$$" ++ pretty n.
+
+Global Instance tmp_var_inj : Inj (=) (=) tmp_var.
+Proof. move => ??. unfold tmp_var => ?. by simplify_eq. Qed.
+
+Module ci2a_linearize.
+
+Inductive error :=
+| UnsupportedExpr (e : static_expr).
+
+Definition M := compiler_monad N (fn_compiler_monoid lexpr) error.
+
+Definition fresh_var : M string :=
+  n ← cget;
+  cput (n + 1)%N;;
+  mret (tmp_var n).
+
+Fixpoint pass (e : static_expr) : M var_val :=
+  match e with
+  | SVar v => mret $ VVar v
+  | SVal v => mret $ VVal v
+  | SBinOp e1 o e2 =>
+      v1 ← pass e1;
+      v2 ← pass e2;
+      v ← fresh_var;
+      cappend (λ x, LLetE v (LBinOp v1 o v2) x);;
+      mret $ VVar v
+  | SLoad e1 =>
+      v1 ← pass e1;
+      v ← fresh_var;
+      cappend (λ x, LLetE v (LLoad v1) x);;
+      mret $ VVar v
+  | SStore e1 e2 =>
+      v1 ← pass e1;
+      v2 ← pass e2;
+      v ← fresh_var;
+      cappend (λ x, LLetE v (LStore v1 v2) x);;
+      mret $ VVar v
+  | SCall f args =>
+      vs ← cmap (pass <$> args) 0 (λ _ a, a);
+      v ← fresh_var;
+      cappend (λ x, LLetE v (LCall f vs) x);;
+      mret $ VVar v
+  | SUbE =>
+      v ← fresh_var;
+      cappend (λ x, LLetE v LUbE x);;
+      mret $ VVar v
+  | SLetE v e1 e2 =>
+      v1 ← pass e1;
+      cappend (λ x, LLetE v (LVarVal v1) x);;
+      pass e2
+  | SIf e1 e2 e3 =>
+      v1 ← pass e1;
+      s ← cget;
+      '(v2, p2) ← cscope (pass e2);
+      '(v3, p3) ← cscope (pass e3);
+      v ← fresh_var;
+      cappend (λ x, LIf (LVarVal v1)
+                        (p2 (LLetE v (LVarVal v2) x))
+                        (p3 (LLetE v (LVarVal v3) x)));;
+      mret $ (VVar v)
+  | _ => cerror (UnsupportedExpr e)
+  end.
+
+Definition test_fn_1 : fndef := {|
+  fd_args := ["x"];
+  fd_body := (BinOp (BinOp (Var "x") ShiftOp (Val 2)) AddOp (Call "f" [Load (Var "x"); Val 1]));
+  fd_static := I;
+|}.
+
+Compute crun 0%N (pass (expr_to_static_expr $ test_fn_1.(fd_body))).
+Compute crun 0%N (pass (expr_to_static_expr $ LetE "v" (BinOp (Val 1) AddOp (Val 1)) $ Var "v")).
+Compute crun 0%N (pass
+                    (expr_to_static_expr $  BinOp
+                       (If (Val 1)
+                           (BinOp (Val 1) AddOp (Val 2))
+                           (Val 3))
+                       AddOp (Var "x"))).
+Compute crun 0%N (pass
+                    (expr_to_static_expr $ BinOp
+                       (If (Val 1)
+                           (BinOp (Val 1) AddOp (Val 2))
+                           (If (Val 1) (Val 2) (Val 3)))
+                       AddOp (Var "x"))).
+
+Definition lookup_var_val (vs : gmap string val) (v : var_val) : option val :=
+  match v with
+  | VVal v => Some (static_val_to_val v)
+  | VVar v => vs !! v
+  end.
+
+Lemma lookup_var_val_to_expr vs v v' :
+  lookup_var_val vs v = Some v' →
+  subst_map vs (var_val_to_expr v) = Val v'.
+Proof. by destruct v => //= ?; simplify_option_eq. Qed.
+
+Lemma lookup_var_val_to_expr_fmap vs v v' :
+  Forall2 (λ v v', lookup_var_val vs v = Some v') v v' →
+  subst_map vs <$> (var_val_to_expr <$> v) = Val <$> v'.
+Proof. elim => //; csimpl => ???? /lookup_var_val_to_expr -> ? ->. done. Qed.
+
+Lemma lookup_var_val_mono vs vs' v v':
+  lookup_var_val vs v = Some v' →
+  vs ⊆ vs' →
+  lookup_var_val vs' v = Some v'.
+Proof. destruct v => //. simplify_eq/=. apply lookup_weaken. Qed.
+
+Lemma pass_state_mono s es s' ei v :
+  crun s (pass es) = CResult s' ei (CSuccess v) →
+  (s ≤ s')%N.
+Proof.
+  move: s s' ei v. induction es => s s' ei ? /= ?; unfold fresh_var in *; simplify_crun_eq => //.
+  all: repeat (case_match; simplify_crun_eq).
+  all: try pose proof (IHes1 _ _ _ _ ltac:(done)).
+  all: try pose proof (IHes2 _ _ _ _ ltac:(done)).
+  all: try pose proof (IHes3 _ _ _ _ ltac:(done)).
+  all: try pose proof (IHes _ _ _ _ ltac:(done)).
+  all: try lia.
+  move: 0%nat H0 => m.
+  elim: H s x x0 x1 m. { move => *; simplify_crun_eq; lia. }
+  move => ?? IH1 ? IH2 *. simplify_crun_eq. move: H => /IH1. move: H0 => /IH2. lia.
+Qed.
+
+
+Local Ltac learn_state :=
+  repeat match goal with
+         | H : crun _ (pass _) = CResult _ _ (CSuccess _) |- _ =>
+             learn_hyp (pass_state_mono _ _ _ _ _ H)
+         end.
+
+Local Ltac prepare_goal :=
+  simplify_eq/=;
+  repeat match goal with
+  | H : ImpExprFill _ _ _ |- _ => destruct H; subst
+  | H : NoDup (_ ++ _) |- _ => apply NoDup_app in H; destruct H as (?&?&?)
+  | H : NoDup (_ :: _) |- _ => apply NoDup_cons in H; destruct H as (?&?)
+  end;
+  unfold fresh_var in *;
+  simplify_crun_eq;
+  repeat (destruct_all!; unfold fresh_var in *; simplify_crun_eq);
+  learn_state.
+
+Lemma pass_correct ei' Ki ei Ks es es' n h fns1 fns2 v s s' vsi vss `{!ImpExprFill es Ks (subst_map vss (static_expr_to_expr es'))}:
+  imp_proof_call n fns1 fns2 →
+  crun s (pass es') = CResult s' ei (CSuccess v) →
+  vss ⊆ vsi →
+  NoDup (assigned_vars (static_expr_to_expr es')) →
+  (∀ n, tmp_var n ∉ assigned_vars (static_expr_to_expr es')) →
+  (∀ v, is_Some (vsi !! v) → v ∉ assigned_vars (static_expr_to_expr es')) →
+  (∀ n, is_Some (vsi !! tmp_var n) → (n < s)%N) →
+  (* TODO: assigned_vars not in vsi and tmp_var greater than n *)
+  (∀ h' v' vsi',
+    (s ≤ s')%N →
+    lookup_var_val vsi' v = Some v' →
+    vsi ⊆ vsi' →
+    (∀ v, is_Some (vsi' !! v) → is_Some (vsi !! v) ∨
+                                v ∈ assigned_vars (static_expr_to_expr es') ∨
+                                ∃ n, v = tmp_var n ∧ (n < s')%N) →
+    Imp (expr_fill Ki $ subst_map vsi' (lexpr_to_expr ei')) h' fns1
+       ⪯{imp_module, imp_module, n, false}
+    Imp (expr_fill Ks (Val v')) h' fns2) →
+  Imp (expr_fill Ki $ subst_map vsi (lexpr_to_expr (ei ei'))) h fns1
+      ⪯{imp_module, imp_module, n, false}
+  Imp es h fns2.
+Proof.
+  move => Hcall.
+  elim: es' es s s' ei ei' v vsi vss h Ks ImpExprFill0; try by move => *; simplify_crun_eq.
+  - move => ?????????????????? Hcont. prepare_goal. case_match. 2: by tstep_s.
+    apply Hcont; [done|by eapply lookup_weaken|done|naive_solver].
+  - move => ?????????????????? Hcont. prepare_goal. apply Hcont; [done|done|done|naive_solver].
+  - move => /= ??? IH1 IH2 ????????????????? Hcont. prepare_goal.
+    eapply IH1; [typeclasses eauto with tstep|done|done|done|set_solver|set_solver|done|].
+    move => ?????? Hvsi'/=.
+    eapply IH2; [typeclasses eauto with tstep|done|by etrans|done|set_solver|set_unfold; naive_solver lia|set_unfold; naive_solver lia|].
+    move => ?????? Hvsi'' /=.
+    erewrite lookup_var_val_to_expr; [|by apply: lookup_var_val_mono].
+    erewrite lookup_var_val_to_expr; [|done].
+    tstep_s => ??.
+    tstep_i. split!.
+    tstep_i. rewrite -subst_subst_map_delete.
+    apply: tsim_mono_b. apply: Hcont.
+    + lia.
+    + by simplify_map_eq.
+    + etrans; [done|]. etrans; [done|]. apply insert_subseteq.
+      apply eq_None_not_Some => /Hvsi''. set_unfold; naive_solver lia.
+    + move => ? /lookup_insert_is_Some'[|]; [naive_solver lia|].
+      move => /Hvsi'' [|[?|?]]; [ |set_unfold; naive_solver lia..].
+      move => /Hvsi'; set_unfold; naive_solver lia.
+  - move => /= ? IH ????????????????? Hcont. prepare_goal.
+    eapply IH; [typeclasses eauto with tstep|done|done|done|set_solver|set_solver|done|].
+    move => ?????? Hvsi'/=.
+    erewrite lookup_var_val_to_expr; [|done].
+    tstep_s => ????. subst.
+    tstep_i. split!.
+    tstep_i. rewrite -subst_subst_map_delete.
+    apply: tsim_mono_b. apply: Hcont.
+    + lia.
+    + by simplify_map_eq.
+    + etrans; [done|]. apply insert_subseteq.
+      apply eq_None_not_Some => /Hvsi'. set_unfold; naive_solver lia.
+    + move => ? /lookup_insert_is_Some'[|]; [naive_solver lia|].
+      move => /Hvsi'; set_unfold; naive_solver lia.
+  - move => /= ?? IH1 IH2 ????????????????? Hcont. prepare_goal.
+    eapply IH1; [typeclasses eauto with tstep|done|done|done|set_solver|set_solver|done|].
+    move => ?????? Hvsi'/=.
+    eapply IH2; [typeclasses eauto with tstep|done|by etrans|done|set_solver|set_unfold; naive_solver lia|set_unfold; naive_solver lia|].
+    move => ?????? Hvsi'' /=.
+    erewrite lookup_var_val_to_expr; [|by apply: lookup_var_val_mono].
+    erewrite lookup_var_val_to_expr; [|done].
+    tstep_s => ???. subst.
+    tstep_i. split!.
+    tstep_i. rewrite -subst_subst_map_delete.
+    apply: tsim_mono_b. apply: Hcont.
+    + lia.
+    + by simplify_map_eq.
+    + etrans; [done|]. etrans; [done|]. apply insert_subseteq.
+      apply eq_None_not_Some => /Hvsi''. set_unfold; naive_solver lia.
+    + move => ? /lookup_insert_is_Some'[|]; [naive_solver lia|].
+      move => /Hvsi'' [|[?|?]]; [ |set_unfold; naive_solver lia..].
+      move => /Hvsi'; set_unfold; naive_solver lia.
+  - move => ??? IH1 IH2 IH3 > ?????? Hcont. prepare_goal.
+    eapply IH1; [typeclasses eauto with tstep|done|done|done|set_solver|set_solver|done|].
+    move => ?????? Hvsi'/=.
+    erewrite lookup_var_val_to_expr; [|done].
+    tstep_s => ??. subst.
+    tstep_i. apply tsim_mono_b_false. case_match.
+    + eapply IH2; [typeclasses eauto with tstep|done|by etrans|done|set_solver|set_unfold; naive_solver lia|set_unfold; naive_solver lia|].
+    move => ?????? Hvsi''/=.
+    erewrite lookup_var_val_to_expr; [|by apply: lookup_var_val_mono].
+    tstep_i. rewrite -subst_subst_map_delete.
+    apply: tsim_mono_b. apply: Hcont.
+    * lia.
+    * by simplify_map_eq.
+    * etrans; [done|]. etrans; [done|]. apply insert_subseteq.
+      apply eq_None_not_Some => /Hvsi''. set_unfold; naive_solver lia.
+    * move => ? /lookup_insert_is_Some'[|]; [naive_solver lia|].
+      move => /Hvsi'' [|[?|?]]; [ |set_unfold; naive_solver lia..].
+      move => /Hvsi'; set_unfold; naive_solver lia.
+    + eapply IH3; [typeclasses eauto with tstep|done|by etrans|done|set_solver|set_unfold; naive_solver lia|set_unfold; naive_solver lia|].
+      move => ?????? Hvsi''/=.
+      erewrite lookup_var_val_to_expr; [|by apply: lookup_var_val_mono].
+      tstep_i. rewrite -subst_subst_map_delete.
+      apply: tsim_mono_b. apply: Hcont.
+      * lia.
+      * by simplify_map_eq.
+      * etrans; [done|]. etrans; [done|]. apply insert_subseteq.
+        apply eq_None_not_Some => /Hvsi''. set_unfold; naive_solver lia.
+      * move => ? /lookup_insert_is_Some'[|]; [naive_solver lia|].
+        move => /Hvsi'' [|[?|?]]; [ |set_unfold; naive_solver lia..].
+        move => /Hvsi'; set_unfold; naive_solver lia.
+  - move => ??? IH1 IH2 ????????????????? Hcont. prepare_goal.
+    eapply IH1; [typeclasses eauto with tstep|done|done|done|set_solver|set_solver|done|].
+    move => ?????? Hvsi'/=. erewrite lookup_var_val_to_expr; [|done].
+    tstep_s. tstep_i. rewrite -!subst_subst_map_delete. apply tsim_mono_b_false.
+    eapply IH2; [typeclasses eauto with tstep|done| |done|set_solver| | |].
+    { by apply insert_mono; etrans. }
+    { move => ?/lookup_insert_is_Some'. set_solver. }
+    { move => ?/lookup_insert_is_Some'. set_unfold; naive_solver lia. }
+    move => ?????? Hvsi''/=.
+    eapply Hcont; [lia|done| |].
+    * etrans; [done|]. etrans; [|done]. apply insert_subseteq.
+      apply eq_None_not_Some => /Hvsi'. set_unfold; naive_solver lia.
+    * move => ? /Hvsi'' [|[?|?]]; [ |set_unfold; naive_solver lia..].
+      move => /lookup_insert_is_Some'[|]; [set_solver|].
+      move => /Hvsi'; set_unfold; naive_solver lia.
+  - move => f args IH es s s' ei ei' v vsi vss h Ks [?] Hrun Hsub Hnodup Htmp Hvsi1 Hvsi2 Hcont. subst.
+    simplify_eq/=. move: Hrun => /cbind_success[s''[p''[v''[?[Hrun ?]]]]]. prepare_goal.
+    move: 0%nat Hrun => m Hrun.
+    change (v'') with ([] ++ v''). move Heqvr'': ([]) => vr''.
+    change (subst_map vss <$> (static_expr_to_expr <$> args)) with ((Val <$> []) ++ (subst_map vss <$> (static_expr_to_expr <$> args))). move Heqva'': ([]) => va''.
+    have Hall : Forall2 (λ vr va, lookup_var_val vsi vr = Some va) vr'' va'' by subst; constructor.
+    clear Heqvr'' Heqva''.
+    elim: IH m p'' v'' s s'' vsi vr'' va'' h Hrun Hsub Hvsi1 Hvsi2 Hnodup Htmp Hall Hcont.
+    + move => /= ??????????????? /lookup_var_val_to_expr_fmap Hall Hcont. simplify_crun_eq. rewrite !app_nil_r.
+      rewrite Hall.
+      apply: Hcall; [typeclasses eauto with tstep|typeclasses eauto with tstep|done| | |done|done|..].
+      { apply Forall2_fmap_l. apply Forall_Forall2_diag. by apply Forall_true. }
+      { apply Forall2_fmap_l. apply Forall_Forall2_diag. by apply Forall_true. }
+      move => ?? /=.
+      tstep_i. rewrite -!subst_subst_map_delete. apply tsim_mono_b_false.
+      apply Hcont.
+      * lia.
+      * by simplify_map_eq.
+      * apply insert_subseteq. apply eq_None_not_Some; naive_solver lia.
+      * move => ? /lookup_insert_is_Some'[|]; naive_solver lia.
+    + csimpl. move => ?? IHe _ IH ???????????????? Hcont. prepare_goal.
+      eapply IHe; [ |done|done|done|set_solver|set_solver|done|].
+      { constructor. by instantiate (1:=(CallCtx _ _ _) ::_). }
+      move => ?????? Hvsi /=. rewrite !cons_middle !app_assoc -fmap_snoc.
+      eapply IH.
+      * done.
+      * by etrans.
+      * set_solver.
+      * set_unfold; naive_solver lia.
+      * done.
+      * set_unfold; naive_solver lia.
+      * apply Forall2_app; [|by econs].
+        apply: Forall2_impl; [done|] => ?? /=?. apply: lookup_var_val_mono; [done|]. by etrans.
+      * move => ?????? Hvsi'. apply Hcont; [lia|done|by etrans|].
+        move => ? /Hvsi'[|]; [| set_unfold; naive_solver lia].
+        move => /Hvsi. set_unfold; naive_solver lia.
+  - move => *. prepare_goal. by tstep_s.
+Qed.
+
+Definition translate_fn (f : static_fndef) : compiler_success lfndef error :=
+  let x := crun 0%N (pass f.(sfd_body)) in
+  match x.(c_result) with
+  | CSuccess v => CSuccess {|
+     lfd_args := f.(sfd_args);
+     lfd_body := x.(c_prog) (LEnd $ LVarVal v);
+  |}
+  | CError e => CError e
+  end.
+
+Compute translate_fn (fndef_to_static_fndef test_fn_1).
+
+Lemma translate_fn_correct f fn fn' :
+  translate_fn fn = CSuccess fn' →
+  NoDup (sfd_args fn ++ assigned_vars (static_expr_to_expr (sfd_body fn))) →
+  (∀ n, tmp_var n ∉ sfd_args fn ++ assigned_vars (static_expr_to_expr (sfd_body fn))) →
+  trefines (MS imp_module (initial_imp_lstate (<[f := fn']> ∅)))
+           (MS imp_module (initial_imp_sstate (<[f := fn]> ∅))).
+Proof.
+  destruct (crun 0%N (pass (sfd_body fn))) as [?? res] eqn: Hsucc.
+  unfold translate_fn. case_match as H => // ? /NoDup_app[?[??]]?. rewrite Hsucc in H. simplify_eq/=.
+  apply imp_proof. { move => ?. rewrite !lookup_fmap !fmap_None !lookup_insert_None. naive_solver. }
+  move => ???????. rewrite !fmap_insert !fmap_empty /=.
+  move => /lookup_insert_Some[[??]|[??]]; simplify_map_eq. split!.
+  move => ?? Hret.
+  rewrite !subst_l_subst_map; [|lia..]. rewrite {1}Hsucc /=.
+  apply: pass_correct; [typeclasses eauto with tstep|done|done|done|done|set_solver|..].
+  { move => ?. rewrite list_to_map_lookup_is_Some. move => [? /(elem_of_zip_l _ _ _)]. set_solver. }
+  { move => ?. rewrite list_to_map_lookup_is_Some. move => [? /(elem_of_zip_l _ _ _)]. set_solver. }
+  move => /= ???????.
+  erewrite lookup_var_val_to_expr; [|done]. by apply Hret.
+Qed.
+
+End ci2a_linearize.
